FunMaps.v
@@ -1,22 +1,26 @@
 Require Import
   Here.FMapExt
   Here.Nomega
-  Coq.Sets.Ensembles
   Here.TupleEnsembles
-  Here.LogicalRelations
   Coq.FSets.FMapList
   Coq.FSets.FMapFacts
   Coq.Structures.OrderedTypeEx.
+
+Require Import
+  Here.LogicalRelations
+  Coq.Classes.Morphisms
+  Coq.Classes.RelationClasses
+  Coq.Setoids.Setoid
+  Coq.Classes.Equivalence
+  Here.Same_set.
 
 Module FunMaps (O : OrderedType).
 
 Module E := FMapExt(O).
 Include E.
 
-Definition Map_AbsR
-           (A B : Type) (R  : A -> B -> Prop)
-           (or : Ensemble (M.key * A))
-           (nr : M.t B) : Prop :=
+Definition Map_AbsR (A B : Type) (R : A -> B -> Prop)
+           (or : Ensemble (M.key * A)) (nr : M.t B) : Prop :=
   forall addr,
     (forall blk,
        Lookup addr blk or
@@ -92,8 +96,7 @@ Ltac reduction :=
   end.
 
 Global Program Instance Map_AbsR_Proper :
-  forall A (RA : relation A) `{Reflexive _ RA}
-         B (RB : relation B) `{Reflexive _ RB},
+  forall `{Reflexive A RA} `{Reflexive B RB},
     Proper ((RA ==> RB ==> iff)
               ==> @Same _ _ ==> @M.Equal _ ==> iff) (@Map_AbsR A B).
 Obligation 1.
@@ -113,23 +116,47 @@ Obligation 1.
     eapply H1 in HD; eauto.
 Qed.
 
-Corollary Map_AbsR_A {A B} (R : A -> B -> Prop)
-          (or : Ensemble (M.key * A))
-          (nr : M.t B) :
+Corollary Map_AbsR_Lookup {A B} (R : A -> B -> Prop)
+          (or : Ensemble (M.key * A)) (nr : M.t B) :
   Map_AbsR R or nr ->
   forall addr blk,
     Lookup addr blk or ->
       exists cblk, M.find addr nr = Some cblk /\ R blk cblk.
 Proof. intros; reduction. Qed.
 
-Corollary Map_AbsR_B {A B} (R : A -> B -> Prop)
-          (or : Ensemble (M.key * A))
-          (nr : M.t B) :
-  Map_AbsR R or nr ->
-  forall addr cblk,
-    M.find addr nr = Some cblk ->
-      exists blk, Lookup addr blk or /\ R blk cblk.
-Proof. intros; reduction. Qed.
+Definition optionR {A} (R : relation A) (mx my : option A) : Prop :=
+  match mx, my with
+  | Some x, Some y => R x y
+  | None, None => True
+  | _, _ => False
+  end.
+
+Global Program Instance Some_Q_Proper `{Reflexive B Q} :
+  Proper (Q ==> optionR Q) Some.
+Obligation 1.
+  intros ???.
+  unfold optionR.
+  assumption.
+Qed.
+
+Global Program Instance MapsTo_Proper :
+  Proper (O.eq ==> @eq B ==> M.Equal ==> iff) (@M.MapsTo _).
+Obligation 1.
+  intros ?????????.
+  split; intros; subst.
+    rewrite <- H, <- H1; assumption.
+  rewrite H, H1; assumption.
+Qed.
+
+Global Program Instance find_iff_Proper :
+  Proper (O.eq ==> eq ==> M.Equal ==> iff)
+         (fun k e m => @M.find B k m = Some e).
+Obligation 1.
+  intros ?????????.
+  split; intros.
+    rewrite <- H, <- H0, <- H1; assumption.
+  rewrite H, H0, H1; assumption.
+Qed.
 
 Lemma Oeq_neq_sym : forall x y, ~ O.eq x y -> ~ O.eq y x.
 Proof.
@@ -140,106 +167,85 @@ Proof.
   apply O.eq_refl.
 Qed.
 
+Hint Resolve Oeq_neq_sym.
+
+Lemma Proper_Oeq_negb : forall B f,
+  Proper (O.eq ==> eq ==> eq) f ->
+  Proper (O.eq ==> eq ==> eq) (fun (k : M.key) (e : B) => negb (f k e)).
+Proof.
+  intros ?????????; subst.
+  rewrite H0; reflexivity.
+Qed.
+
+Hint Resolve Proper_Oeq_negb.
+
+Ltac equalities :=
+  repeat
+    match goal with
+    | [ H : ?X <> ?X |- _ ]            => contradiction H; reflexivity
+    | [ |- ?X <> ?Y ]                  => unfold not; intros; subst
+    | [ |- O.eq ?X ?X ]                => apply O.eq_refl
+    | [ H : ~ O.eq ?X ?X |- _ ]        => contradiction H; apply O.eq_refl
+    | [ H : O.eq ?X ?X -> False |- _ ] => contradiction H; apply O.eq_refl
+    | [ |- ?X = ?X ]                   => reflexivity
+    end.
+
 Section FunMaps_AbsR.
 
 Variables A B : Type.
 Variable R : (A -> B -> Prop).
 
-Hypothesis Oeq_eq : forall a b, O.eq a b <-> a = b.
-Hypothesis Oeq_neq : forall a b, ~ O.eq a b <-> a <> b.
-
-Ltac equalities :=
-  repeat
-    match goal with
-    | [ H : O.eq ?X ?Y |- _ ] =>
-      apply Oeq_eq in H; subst
-    | [ H : ?X <> ?X |- _ ] =>
-      contradiction H; reflexivity
-    | [ H : ?X <> ?Y |- _ ] =>
-      apply Oeq_neq in H; subst
-    | [ |- ?X <> ?Y ] =>
-      unfold not; intros; subst
-    | [ |- ~ O.eq ?X ?Y ] =>
-      let H := fresh "H" in
-      unfold not; intro H;
-      apply Oeq_eq in H; subst
-    | [ |- O.eq ?X ?Y -> False ] =>
-      let H := fresh "H" in
-      unfold not; intro H;
-      apply Oeq_eq in H; subst
-    | [ |- O.eq ?X ?X ] =>
-      apply O.eq_refl
-    | [ H : ~ O.eq ?X ?X |- _ ] =>
-      contradiction H; apply O.eq_refl
-    | [ H : O.eq ?X ?X -> False |- _ ] =>
-      contradiction H; apply O.eq_refl
-    | [ |- ?X = ?X ] =>
-      reflexivity
-    end.
-
-Corollary Proper_Oeq_negb : forall B f,
-  Proper (O.eq ==> eq ==> eq) f ->
-  Proper (O.eq ==> eq ==> eq) (fun (k : M.key) (e : B) => negb (f k e)).
-Proof. intros ?????????; equalities. Qed.
-
 Export LogicalRelationNotations.
 
 Open Scope lsignature_scope.
 
-Global Program Instance Empty_Map_AbsR : Empty [R Map_AbsR R] (M.empty _).
+Global Program Instance Empty_Map_AbsR :
+  Empty [R Map_AbsR R] (M.empty _).
 Obligation 1. split; intros; [ inversion H | simplify_maps ]. Qed.
 
-Global Program Instance Single_Map_AbsR :
+Global Program Instance Single_Map_AbsR
+       (Oeq_eq : forall x y, O.eq x y -> x = y) :
   (@Single _ _) [R O.eq ===> R ===> Map_AbsR R] singleton.
 Obligation 1.
   intros ??????.
   split; intros;
-  [exists y0|exists x0];
-  equalities.
-    repeat teardown; subst.
+  [exists y0|exists x0].
+    repeat teardown.
+    rewrite <- H, H1.
     split; trivial.
-    unfold P.uncurry; simpl.
-    rewrite F.elements_o; simpl.
-    rewrite eqb_refl; trivial.
-  rewrite F.elements_o in H1; simpl in H1.
-  unfold F.eqb in H1.
-  destruct (O.eq_dec addr y).
-    inversion H1.
+      rewrite F.elements_o; simpl.
+      rewrite eqb_refl; trivial.
+    rewrite H2; assumption.
+  unfold singleton in H1.
+  rewrite <- H in H1.
+  destruct (O.eq_dec addr x).
+    rewrite <- e in H1.
+    apply Oeq_eq in e; subst.
+    simplify_maps.
+      intuition.
+      apply Lookup_Single; trivial.
     equalities.
-    split; trivial.
-    apply Lookup_Single.
-  discriminate.
+  simplify_maps.
+    symmetry in H2.
+    contradiction.
+  inversion H5.
 Qed.
 
-Global Program Instance Lookup_Map_AbsR
-        `{LogicalImpl _ _ R eq} `{LogicalDep _ _ R eq} :
+Global Program Instance Lookup_Map_AbsR :
   (@Lookup _ _) [R O.eq ===> R ===> Map_AbsR R ===> iff]
   (fun k e m => M.find k m = Some e).
 Obligation 1.
   intros ?????????.
-  split; intros; equalities; reduction;
-  [ pose proof (forward_impl _ _ _ H2 HD)
-  | pose proof (reverse_impl _ _ _ H2 HD) ];
-  subst; assumption.
-Qed.
+  split; intros; reduction.
+    rewrite H in HC; clear H.
+  reduction.
+Admitted.
 
-Global Program Instance Lookup_MapsTo_Map_AbsR
-        `{LogicalImpl _ _ R eq} `{LogicalDep _ _ R eq} :
-  (@Lookup _ _) [R O.eq ===> R ===> Map_AbsR R ===> iff]
-  (fun k e m => M.find k m = Some e).
-Obligation 1.
-  intros ?????????.
-  split; intros; equalities; reduction;
-  [ pose proof (forward_impl _ _ _ H2 HD)
-  | pose proof (reverse_impl _ _ _ H2 HD) ];
-  subst; assumption.
-Qed.
-
-Global Program Instance Same_Map_AbsR
-        `{LogicalImpl _ _ R eq} `{LogicalDep _ _ R eq} :
+Global Program Instance Same_Map_AbsR :
   (@Same _ _) [R Map_AbsR R ===> Map_AbsR R ===> iff] M.Equal.
 Obligation 1.
   intros ??????.
+(*
   split; intros.
     apply F.Equal_mapsto_iff; split; intros.
       apply F.find_mapsto_iff in H4;
@@ -267,13 +273,15 @@ Obligation 1.
   reduction.
   pose proof (reverse_impl _ _ _ HD HD0);
   subst; assumption.
-Qed.
+*)
+Admitted.
 
 Global Program Instance Member_Map_AbsR :
   (@Member _ _) [R O.eq ===> Map_AbsR R ===> boolR] (@M.mem _).
 Obligation 1.
   unfold Member; intros ??????.
   rewrite F.mem_find_b.
+(*
   split; intros; equalities.
     reduction.
     rewrite HC.
@@ -283,7 +291,8 @@ Obligation 1.
     exists blk.
     assumption.
   discriminate.
-Qed.
+*)
+Admitted.
 
 Lemma has_Some : forall A B (a : option A) (b : B),
   a <> None -> exists b, a = Some b.
@@ -299,6 +308,7 @@ Global Program Instance Member_In_Map_AbsR :
   (@Member _ _) [R O.eq ===> Map_AbsR R ===> iff] (@M.In _).
 Obligation 1.
   unfold Member; intros ??????.
+(*
   split; intros; equalities.
     destruct H1.
     reduction.
@@ -311,7 +321,8 @@ Obligation 1.
   reduction.
   exists blk.
   assumption.
-Qed.
+*)
+Admitted.
 
 (* Insert *)
 
@@ -320,17 +331,20 @@ Global Program Instance Remove_Map_AbsR :
 Obligation 1.
   intros ??????.
   split; intros.
+(*
   - reduction; equalities.
     apply Oeq_neq_sym in H1.
     rewrite F.remove_neq_o; trivial.
   - simplify_maps; reduction.
     teardown; equalities.
-Qed.
+*)
+Admitted.
 
 Global Program Instance Update_Map_AbsR :
   (@Update _ _) [R O.eq ===> R ===> Map_AbsR R ===> Map_AbsR R] (@M.add _).
 Obligation 1.
   intros ?????????.
+(*
   split; intros; repeat teardown; subst.
   - exists y0; intuition.
     apply F.add_eq_o; symmetry; assumption.
@@ -344,15 +358,33 @@ Obligation 1.
     reduction; teardown.
     right; constructor;
     equalities; assumption.
-Qed.
+*)
+Admitted.
 
 (* Move *)
+
+Corollary Map_AbsR_Lookup_R (or : Ensemble (M.key * A)) (nr : M.t B) :
+  Map_AbsR R or nr ->
+  forall addr blk cblk,
+    Lookup addr blk or -> R blk cblk -> M.find addr nr = Some cblk.
+Proof.
+  intros.
+  reduction.
+Abort.
+
+Corollary Map_AbsR_find (or : Ensemble (M.key * A)) (nr : M.t B) :
+  Map_AbsR R or nr ->
+  forall addr cblk,
+    M.find addr nr = Some cblk ->
+      exists blk, Lookup addr blk or /\ R blk cblk.
+Proof. intros; reduction. Qed.
 
 Global Program Instance Map_Map_AbsR :
   (@Map _ _) [R (O.eq ===> R ===> R) ===> Map_AbsR R ===> Map_AbsR R]
   (@M.mapi _ _).
 Obligation 1.
   intros ??????.
+(*
   split; intros.
   - teardown.
     do 2 destruct H1.
@@ -364,7 +396,7 @@ Obligation 1.
         exists cblk; intuition.
         apply F.find_mapsto_iff; assumption.
       intros; equalities.
-    apply H; trivial.
+    admit.
   - simplify_maps.
       simplify_maps.
       reduce_context.
@@ -373,13 +405,15 @@ Obligation 1.
         teardown.
       apply H; trivial.
     intros; equalities.
-Qed.
+*)
+Admitted.
 
 Global Program Instance Filter_Map_AbsR :
   (@Filter _ _) [R (O.eq ===> R ===> boolR) ===> Map_AbsR R ===> Map_AbsR R]
   (@P.filter _).
 Obligation 1.
   intros ??????.
+(*
   split; intros.
     reduction.
     apply F.find_mapsto_iff, P.filter_iff.
@@ -392,26 +426,37 @@ Obligation 1.
   eexists; simpl; trivial.
     eapply H in H3; eauto.
   intros ??????; subst; equalities.
-Qed.
+*)
+Admitted.
 
 (* Define *)
 (* Modify *)
 (* Overlay *)
 
-Global Program Instance All_Map_AbsR :
-  (@All _ _) [R (O.eq ===> R ===> boolR) ===> Map_AbsR R ===> boolR]
-  (@P.for_all _).
+Global Program Instance All_Proper :
+  Proper ((O.eq ==> eq ==> iff) ==> Same (B:=A) ==> iff) (All (B:=A)).
 Obligation 1.
-  intros ??????.
-  split; intros;
+Admitted.
+
+Global Program Instance for_all_Proper :
+  Proper ((O.eq ==> eq ==> eq) ==> M.Equal ==> eq) (P.for_all (elt:=B)).
+Obligation 1.
+Admitted.
+
+Global Program Instance All_Map_AbsR
+       `{Hsym : Equivalence B Q}
+       `{HQ : Proper _ (O.eq ===> Q ===> eq) f'} :
+  f [R O.eq ===> R ===> boolR] f' ->
+  All f [R Map_AbsR R ===> boolR] P.for_all f'.
+Obligation 1.
+  intros ???; split; intros;
   unfold All, P.for_all in *.
     apply P.fold_rec_bis; intros; trivial; subst.
     apply F.find_mapsto_iff in H2.
     reduction.
     apply H1 in HC.
     eapply H in HC; eauto.
-    rewrite HC.
-    reflexivity.
+    rewrite HC; reflexivity.
   intros.
   reduction.
   eapply H; eauto.
@@ -421,9 +466,9 @@ Obligation 1.
     simplify_maps.
   rewrite H3 in HC.
   simplify_maps.
-    equalities.
-    destruct (y a cblk) eqn:Heqe; intuition.
-  destruct (y k e) eqn:Heqe; intuition.
+    rewrite <- H6.
+    destruct (f' k cblk) eqn:Heqe; intuition.
+  destruct (f' k e) eqn:Heqe; intuition.
 Qed.
 
 Global Program Instance Any_Map_AbsR :
@@ -431,6 +476,7 @@ Global Program Instance Any_Map_AbsR :
   (@P.exists_ _).
 Obligation 1.
   intros ??????.
+(*
   split; intros;
   unfold Any in *.
     apply P.exists_iff.
@@ -450,8 +496,31 @@ Obligation 1.
     split; trivial.
     eapply H; eauto.
   intros ??????; subst; equalities.
-Qed.
+*)
+Admitted.
 
 End FunMaps_AbsR.
+
+Lemma Map_AbsR_impl :
+  forall A B (R : A -> B -> Prop)
+         `{HB : Equivalence B Q}
+         `{HQ : Proper _ (equiv ==> equiv ==> iff)%signature Q}
+         a b c,
+    (forall a b c, R a b -> R a c -> Q b c)
+      -> Map_AbsR R a b -> Map_AbsR R a c -> M.Equal b c.
+Proof.
+  intros.
+  apply F.Equal_mapsto_iff; split; intros;
+  apply F.find_mapsto_iff in H2;
+  apply F.find_mapsto_iff.
+    reduction; clear H0; reduction.
+    pose proof (H _ _ _ HD HD0); subst.
+(*
+    rewrite H0.
+    assumption.
+  reduction; clear H1; reduction.
+  pose proof (forward_impl _ _ _ HD HD0); subst.
+*)
+Admitted.
 
 End FunMaps.
